examples/concurrency-strategies/commutativity-strategy.dfy
@@ -1,4 +1,30 @@
 include "spec.s.dfy"
 
 module TheoremProof {
+
+  lemma Correctness(b:Behavior<Concrete.State>, I:CState->AState)
+    requires Reachable(b, Concrete.Init, Concrete.Next)
+    ensures var ab := Interpret(b, I); Reachable(ab, Abstract.Init, Abstract.Next)
+  {
+    var ab := Interpret(b, I);
+
+    if (b is in the good TLA order) {
+      call the tla refinement proof
+    } else {
+      pick an index very carefully:
+        - terminates
+        - can satisfy ind. hyp.
+      var b' := swap(b, idx)
+      assert Reachable(b', Concrete.Init, Concrete.Next);
+ 
+      var ab' := Interpret(b', I);  // required by spec
+      Correctness(b', I);
+      assert Reachable(ab', Abstract.Init, Abstract.Next);
+
+
+      assert Reachable(ab, Abstract.Init, Abstract.Next);
+    }
+  }
+  
+
 }
